kore/src/Basics.v
@@ -355,3 +355,4 @@ match x with
 | None   => y
 end.
 Notation "f <|> g" := (orElse f g) (at level 56, left associativity).
+
